theories/heap_lang/adequacy.v
@@ -1,54 +1,54 @@
 From iris.proofmode Require Import tactics.
 From iris.algebra Require Import auth.
 From iris.base_logic.lib Require Import proph_map.
-From iris.program_logic Require Import weakestpre adequacy hoare.
+From iris.program_logic Require Import weakestpre adequacy.
 From intensional.heap_lang Require Import lang proofmode notation.
 Set Default Proof Using "Type".
 
-Class heapPreG Σ := HeapPreG {
-  heap_preG_iris :> invPreG Σ;
-  heap_preG_heap :> gen_heapPreG loc val Σ;
-  heap_preG_proph :> proph_mapPreG proph_id (val * val) Σ;
+Class heapGpreS Σ := HeapGpreS {
+  heap_preG_iris :> invGpreS Σ;
+  heap_preG_heap :> gen_heapGpreS loc val Σ;
+  heap_preG_proph :> proph_mapGpreS proph_id (val * val) Σ;
   heap_preG_trace :> trace_preG Σ;
 }.
 
 Definition heapΣ : gFunctors := #[invΣ; gen_heapΣ loc val; proph_mapΣ proph_id (val * val); traceΣ].
-Instance subG_heapPreG {Σ} : subG heapΣ Σ → heapPreG Σ.
+Instance subG_heapPreG {Σ} : subG heapΣ Σ → heapGpreS Σ.
 Proof. solve_inG. Qed.
 
-Definition heap_adequacy Σ `{!heapPreG Σ} s e σ φ :
-  (∀ `{!heapG Σ}, ⊢ WP e @ s; ⊤ {{ v, ⌜φ v⌝ }}) →
+Definition heap_adequacy Σ `{!heapGpreS Σ} s e σ φ :
+  (∀ `{!heapGS Σ}, ⊢ WP e @ s; ⊤ {{ v, ⌜φ v⌝ }}) →
   adequate s e σ (λ v _, φ v).
 Proof.
   intros Hwp; eapply (wp_adequacy _ _); iIntros (??) "".
-  iMod (gen_heap_init σ.(heap)) as (?) "Hh".
+  iMod (gen_heap_init σ.(heap)) as (?) "[Hh _]".
   iMod (proph_map_init κs σ.(used_proph_id)) as (?) "Hp".
   iMod (trace_auth_init σ.(trace)) as (?) "(Ht & _ & _)".
   iModIntro. iExists
-    (λ σ κs, (gen_heap_ctx σ.(heap) ∗ trace_auth σ.(trace) ∗ proph_map_ctx κs σ.(used_proph_id))%I),
+    (λ σ κs, (gen_heap_interp σ.(heap) ∗ trace_auth σ.(trace) ∗ proph_map_interp κs σ.(used_proph_id))%I),
     (λ _, True%I).
-  iFrame. iApply (Hwp (HeapG _ _ _ _ _)).
+  iFrame. iApply (Hwp (HeapGS _ _ _ _ _)).
 Qed.
 
-Definition heap_invariance Σ `{!heapPreG Σ} (N: namespace) (I: list val → Prop) s e σ :
+Definition heap_invariance Σ `{!heapGpreS Σ} (N: namespace) (I: list val → Prop) s e σ :
   I (trace σ) →
-  (∀ `{!heapG Σ}, ⊢ trace_inv N I -∗ trace_is (trace σ) -∗ WP e @ s; ⊤ {{ _, True }}) →
+  (∀ `{!heapGS Σ}, ⊢ trace_inv N I -∗ trace_is (trace σ) -∗ WP e @ s; ⊤ {{ _, True }}) →
   ∀ σ' t,
     rtc erased_step ([e], σ) (t, σ') →
     I (trace σ').
 Proof.
   intros HI Hwp σ' t.
   eapply (wp_invariance Σ _ s _ _ _ _ (I (trace σ'))). iIntros (Hinv κs) "".
-  iMod (gen_heap_init σ.(heap)) as (?) "Hh".
+  iMod (gen_heap_init σ.(heap)) as (?) "[Hh _]".
   iMod (proph_map_init κs σ.(used_proph_id)) as (?) "Hp".
   iMod (trace_auth_init σ.(trace)) as (?) "(Hta & Ht & Hth)".
   iDestruct (inv_alloc N _ (∃ t, trace_half_frag t ∗ ⌜I t⌝) with "[Hth]") as ">#HI".
   { iNext. eauto. }
   iModIntro. iExists
-    (λ σ κs _, (gen_heap_ctx σ.(heap) ∗ trace_auth σ.(trace) ∗ proph_map_ctx κs σ.(used_proph_id))%I),
+    (λ σ κs _, (gen_heap_interp σ.(heap) ∗ trace_auth σ.(trace) ∗ proph_map_interp κs σ.(used_proph_id))%I),
     (λ _, True%I).
   iFrame. iSplitL.
-  { iDestruct (Hwp (HeapG _ _ _ _ _)) as "Hwp". iApply ("Hwp" with "HI Ht"). }
+  { iDestruct (Hwp (HeapGS _ _ _ _ _)) as "Hwp". iApply ("Hwp" with "HI Ht"). }
   iIntros "(_ & Hta & _)". iExists _.
   iInv "HI" as ">Ht'" "_". iDestruct "Ht'" as (t') "(Ht' & %)".
   iDestruct (trace_auth_half_frag_agree with "Hta Ht'") as %->. iModIntro. eauto.
@@ -66,8 +66,8 @@ Qed.
    from the paper, as we only require the trace property to hold of the trace of
    the initial state σ, while the theorem in the paper is specialized to the
    case where the initial trace is the empty trace. *)
-Lemma module_invariance {Σ} `{heapPreG Σ} (N: namespace)
-  (Φ: ∀ `{heapG Σ}, iProp Σ → val → iProp Σ)  (* Module specification *)
+Lemma module_invariance {Σ} `{heapGpreS Σ} (N: namespace)
+  (Φ: ∀ `{heapGS Σ}, iProp Σ → val → iProp Σ)  (* Module specification *)
   (P0: iProp Σ) (* Initial resources required by the module *)
   (e: val → expr) (* Context program, parameterized by the module *)
   (e_init: expr) (* Initialization code, used to allocate resources for P0 *)
@@ -78,12 +78,12 @@ Lemma module_invariance {Σ} `{heapPreG Σ} (N: namespace)
   (* The initial trace must satisfy the property *)
   good_trace (trace σ) →
   (* The context must be safe, given a module satisfying the specification Φ *)
-  (⊢ ∀ `(heapG Σ) P m, Φ P m -∗ {{{ P }}} e m {{{ v, RET v; True }}}) →
+  (⊢ ∀ `(heapGS Σ) P m, Φ P m -∗ {{{ P }}} e m {{{ v, RET v; True }}}) →
   (* The initialization code must provide P0 *)
-  (⊢ ∀ `(heapG Σ), {{ True }} e_init {{ _, P0 }}) →
+  (⊢ ∀ `(heapGS Σ), {{{ True }}} e_init {{{ v, RET v; P0 }}}) →
   (* The implementation provided for the module (iops) must satisfy the specification Φ.
      On top of P0 it is given SL resources for the trace. *)
-  (⊢ ∀ `(heapG Σ), Φ (P0 ∗ trace_is (trace σ) ∗ trace_inv N good_trace)%I imimpl) →
+  (⊢ ∀ `(heapGS Σ), Φ (P0 ∗ trace_is (trace σ) ∗ trace_inv N good_trace)%I imimpl) →
   (* Then the trace remains good at every step *)
   ∀ σ' e',
     rtc erased_step ([(e_init;; e imimpl)%E], σ) (e', σ') →
@@ -91,9 +91,8 @@ Lemma module_invariance {Σ} `{heapPreG Σ} (N: namespace)
 Proof.
   intros Htrσ Hctx Hinit Himpl σ' e' Hsteps.
   eapply heap_invariance. done. by apply Htrσ. 2: eapply Hsteps.
-  iIntros (?) "HI Htr". wp_bind e_init.
-  iApply wp_wand. by iApply Hinit.
-  iIntros (v) "H0". wp_pures.
+  iIntros (?) "HI Htr". wp_bind e_init. iApply Hinit. done.
+  iIntros "!>" (v) "H0". wp_pures.
   iApply (Hctx with "[] [H0 Htr HI]").
   - iApply Himpl.
   - iFrame.
